LÃ¶sen Sie nach den jeweils gesuchten Variablen auf:

::: {.content-hidden when-profile="solved" unless-meta="hide-solutions.101010"}
#. $t$ ist gesucht

   $K_t=K_0 \cdot (1+i)^t$

#. $i$ ist gesucht

   $K_t=K_0 \cdot (1+i)^t$

#. $x$ ist gesucht

   $(x-7) \cdot (x+2)=0$

#. $x$ ist gesucht

   $\sqrt{x+2}=4$
:::

::: {.content-visible when-profile="solved" unless-meta="hide-solutions.101010"}
#. $t$ ist gesucht

   $K_t=K_0 \cdot (1+i)^t$ $\mid :K_0$

   $\frac{K_t}{K_0}=(1+i)^t$ $\mid \ln$

   $\ln(\frac{K_t}{K_0})=\ln((1+i)^t)$ $\mid$ Logarithmengesetz

   $\ln(\frac{K_t}{K_0})=t \cdot \ln(1+i)$ $\mid :\ln(1+i)$

   $t=\frac{\ln(\frac{K_t}{K_0})}{\ln(1+i)}$

#. $i$ ist gesucht

   $K_t=K_0 \cdot (1+i)^t$ $\mid :K_0$

   $\frac{K_t}{K_0}=(1+i)^t$ $\mid \sqrt[t]{}$

   $\sqrt[t]{\frac{K_t}{K_0}}=1+i$ $\mid -1$

   oder $i=\sqrt[t]{\frac{K_t}{K_0}}-1$

#. $x$ ist gesucht

   $(x-7) \cdot (x+2)=0$

   $x-7=0$

   $x_1=7$

   oder $x+2=0$

   $x_2=-2$

#. $x$ ist gesucht

   $\sqrt{x+2}=4$ $\mid ()^2$

   $x+2=4^2$ $\mid -2$

   $x=14$

{{< pagebreak >}}
:::
